rename callproof -> mk_annot

ImpMonads.v
@@ -17,7 +17,7 @@ Module Type MayReturnMonad.
 
   Axiom bind: forall {A B}, (t A) -> (A -> t B) -> t B.
 
-  Axiom callproof: forall {A} (k: t A), t { a: A | mayRet k a }.
+  Axiom mk_annot: forall {A} (k: t A), t { a: A | mayRet k a }.
 
   Axiom mayRet_ret: forall A (a b:A), 
      mayRet (ret a) b -> a=b.
@@ -43,8 +43,8 @@ Module Type MayReturnMonad.
   Axiom impeq_bind_assoc: forall (A B C:Type) (k1: t A) (k2: A -> t B) (k3: B -> t C),
      (impeq (bind (bind k1 k2) (fun b => k3 b)) (bind k1 (fun a => bind (k2 a) (fun b => k3 b)))).
 
-  Axiom impeq_bind_callproof: forall (A:Type) (k: t A),
-     (impeq (bind (callproof k) (fun a => ret (proj1_sig a))) k).
+  Axiom impeq_bind_mk_annot: forall (A:Type) (k: t A),
+     (impeq (bind (mk_annot k) (fun a => ret (proj1_sig a))) k).
 
 End MayReturnMonad.
 
@@ -62,7 +62,7 @@ Module PowerSetMonad<: MayReturnMonad.
    Definition bind {A B:Type} (k1: t A) (k2: A -> t B) := 
      fun b => exists a, k1 a /\ k2 a b.
 
-   Definition callproof {A} (k: t A) : t { a | mayRet k a } := fun _ => True.
+   Definition mk_annot {A} (k: t A) : t { a | mayRet k a } := fun _ => True.
 
    Lemma mayRet_ret A (a b:A): mayRet (ret a) b -> a=b.
    Proof.
@@ -114,10 +114,10 @@ Module PowerSetMonad<: MayReturnMonad.
      unfold impeq, bind, ret; firstorder (subst; auto).
    Qed.
 
-   Lemma impeq_bind_callproof: forall (A:Type) (k: t A),
-     (impeq (bind (callproof k) (fun a => ret (proj1_sig a))) k).
+   Lemma impeq_bind_mk_annot: forall (A:Type) (k: t A),
+     (impeq (bind (mk_annot k) (fun a => ret (proj1_sig a))) k).
    Proof.
-     unfold impeq, bind, ret, callproof, mayRet. intros A k a; constructor 1.
+     unfold impeq, bind, ret, mk_annot, mayRet. intros A k a; constructor 1.
      - intros [[x H] [H0 H1]]. subst; simpl; auto.
      - intros. constructor 1 with (x:=(exist _ _ H)). simpl; intuition.
    Qed.
@@ -137,7 +137,7 @@ Module TrivialMonad<: MayReturnMonad.
 
    Definition bind {A B:Type} (k1: A) (k2: A -> B) := k2 k1.
 
-   Definition callproof {A} (k: t A) : t { a: A | mayRet k a } 
+   Definition mk_annot {A} (k: t A) : t { a: A | mayRet k a } 
     := exist _ k (eq_refl k) .
 
    Lemma mayRet_ret (A:Type) (a b:A): mayRet (ret a) b -> a=b.
@@ -189,10 +189,10 @@ Module TrivialMonad<: MayReturnMonad.
      unfold impeq, bind, ret; firstorder (subst; auto).
    Qed.
 
-   Lemma impeq_bind_callproof: forall (A:Type) (k: t A),
-     (impeq (bind (callproof k) (fun a => ret (proj1_sig a))) k).
+   Lemma impeq_bind_mk_annot: forall (A:Type) (k: t A),
+     (impeq (bind (mk_annot k) (fun a => ret (proj1_sig a))) k).
    Proof.
-     unfold impeq, bind, ret, callproof, mayRet. simpl. auto.
+     unfold impeq, bind, ret, mk_annot, mayRet. simpl. auto.
    Qed.
 
 End TrivialMonad.
@@ -215,7 +215,7 @@ Module StateMonad<: MayReturnMonad.
    Definition bind {A B:Type} (k1: t A) (k2: A -> t B) := 
      fun s0 => let r := k1 s0 in k2 (fst r) (snd r).
 
-   Program Definition callproof {A} (k: t A) : t { a | mayRet k a } := 
+   Program Definition mk_annot {A} (k: t A) : t { a | mayRet k a } := 
      fun s0 => let r := k s0 in (exist _ (fst r) _, snd r).
    Obligation 1.
      unfold mayRet; eauto.
@@ -272,10 +272,10 @@ Module StateMonad<: MayReturnMonad.
      unfold impeq, bind, ret. auto.
    Qed.
 
-   Lemma impeq_bind_callproof: forall (A:Type) (k: t A),
-     (impeq (bind (callproof k) (fun a => ret (proj1_sig a))) k).
+   Lemma impeq_bind_mk_annot: forall (A:Type) (k: t A),
+     (impeq (bind (mk_annot k) (fun a => ret (proj1_sig a))) k).
    Proof.
-     unfold impeq, bind, ret, callproof, mayRet.  simpl. intros A k s; destruct k; simpl; auto.
+     unfold impeq, bind, ret, mk_annot, mayRet.  simpl. intros A k s; destruct k; simpl; auto.
    Qed.
 
 End StateMonad.
