ImpIO.v
@@ -82,10 +82,10 @@ Qed.
 
 Program Definition try_with_fail_ensure {A} (k1: unit -> ?? A) (k2: pstring -> exn -> ??A) (P: A -> Prop | wlp (k1 tt) P /\ (forall s e, wlp (k2 s e) P)): ?? { r | P r }
   := TRY
-        DO r <~ callproof (k1 tt);; 
+        DO r <~ mk_annot (k1 tt);; 
         RET (exist P r _)
      WITH_FAIL s, e => 
-        DO r <~ callproof (k2 s e);;
+        DO r <~ mk_annot (k2 s e);;
         RET (exist P r _).
 Obligation 2.
   unfold wlp in * |- *; eauto.
